Load and cast-load lemmas are added. Efield_denote is split into new efield_denote and tc_efield. Side conditions in floyd is rearranged. Progs folder words as it did. If Andrew is working on sha, some small modification on typechecking might be necessary, though no modification in progs is required.

floyd/loadstore_field_at.v
@@ -62,6 +62,7 @@ Inductive efield : Type :=
   | eArraySubsc: forall i: expr, efield
   | eStructField: forall i: ident, efield
   | eUnionField: forall i: ident, efield.
+(* Maybe it should be moved to nested_field_lemmas. But maybe not. *)
 
 Fixpoint nested_efield (e: expr) (efs: list efield) (tts: list type) : expr :=
   match efs, tts with
@@ -98,19 +99,29 @@ Definition compute_lr e (efs: list efield) :=
   | _, _ => LLLL
   end.
 
-Fixpoint efield_denote (Delta: tycontext) (efs: list efield) (gfs: list gfield) : environ -> mpred :=
+Fixpoint efield_denote (efs: list efield) (gfs: list gfield) : environ -> mpred :=
   match efs, gfs with
   | nil, nil => TT
   | eArraySubsc ei :: efs', ArraySubsc i :: gfs' => 
     local (`(eq (Vint (Int.repr i))) (eval_expr ei)) &&
     !! (match typeof ei with | Tint _ _ _ => True | _ => False end) &&
-    local (tc_expr Delta ei) &&
-    efield_denote Delta efs' gfs'
+    efield_denote efs' gfs'
   | eStructField i :: efs', StructField i0 :: gfs' =>
-    !! (i = i0) && efield_denote Delta efs' gfs'
+    !! (i = i0) && efield_denote efs' gfs'
   | eUnionField i :: efs', UnionField i0 :: gfs' =>
-    !! (i = i0) && efield_denote Delta efs' gfs'
+    !! (i = i0) && efield_denote efs' gfs'
   | _, _ => FF
+  end.
+
+Fixpoint tc_efield (Delta: tycontext) (efs: list efield) rho : Prop :=
+  match efs with
+  | nil => True
+  | eArraySubsc ei :: efs' => 
+    tc_expr Delta ei rho /\ tc_efield Delta efs' rho
+  | eStructField i :: efs' =>
+    tc_efield Delta efs' rho
+  | eUnionField i :: efs' =>
+    tc_efield Delta efs' rho
   end.
 
 (*
@@ -193,7 +204,7 @@ Qed.
 
 Lemma typeof_nested_efield: forall env Delta t_root e efs gfs tts lr,
   legal_nested_efield env t_root e gfs tts lr = true ->
-  efield_denote Delta efs gfs |--
+  local (tc_efield Delta efs) && efield_denote efs gfs |--
     !! (uncompomize env (nested_field_type2 t_root gfs) = typeof (nested_efield e efs tts)).
 Proof.
 Admitted.
@@ -432,8 +443,9 @@ Definition tc_LR Delta e lr :=
 
 Lemma eval_lvalue_nested_efield_aux: forall Delta env t_root e efs gfs tts lr,
   legal_nested_efield env t_root e gfs tts lr = true ->
-  local (`isptr (eval_LR e lr)) && local (tc_LR Delta e lr) && efield_denote Delta efs gfs |--
-    local (`isptr (eval_lvalue (nested_efield e efs tts))) &&
+  local (`isptr (eval_LR e lr)) && local (tc_LR Delta e lr) &&
+    local (tc_efield Delta efs) && efield_denote efs gfs |--
+  local (`isptr (eval_lvalue (nested_efield e efs tts))) &&
     local (tc_lvalue Delta (nested_efield e efs tts)) &&
     local (`eq (eval_lvalue (nested_efield e efs tts))
       (`(field_address t_root gfs) (eval_LR e lr))).
@@ -565,7 +577,8 @@ Qed.
 
 Lemma eval_lvalue_nested_efield: forall Delta env t_root e efs gfs tts lr,
   legal_nested_efield env t_root e gfs tts lr = true ->
-  local (`isptr (eval_LR e lr)) && local (tc_LR Delta e lr) && efield_denote Delta efs gfs |-- local (`eq (eval_lvalue (nested_efield e efs tts))
+  local (`isptr (eval_LR e lr)) && local (tc_LR Delta e lr) &&
+  local (tc_efield Delta efs) && efield_denote efs gfs |-- local (`eq (eval_lvalue (nested_efield e efs tts))
       (`(field_address t_root gfs) (eval_LR e lr))).
 Proof.
   intros.
@@ -575,7 +588,8 @@ Qed.
 
 Lemma tc_lvalue_nested_efield: forall Delta env t_root e efs gfs tts lr,
   legal_nested_efield env t_root e gfs tts lr = true ->
-  local (`isptr (eval_LR e lr)) && local (tc_LR Delta e lr) && efield_denote Delta efs gfs |--
+  local (`isptr (eval_LR e lr)) && local (tc_LR Delta e lr) &&
+  local (tc_efield Delta efs) && efield_denote efs gfs |--
     local (`isptr (eval_lvalue (nested_efield e efs tts))) &&
     local (tc_lvalue Delta (nested_efield e efs tts)).
 Proof.
@@ -596,7 +610,8 @@ Lemma semax_max_path_field_load_37':
       PROPx P (LOCALx (tc_environ Delta :: Q) (SEPx R)) |--
         local (tc_LR Delta e1 lr) &&
         local `(tc_val (typeof (nested_efield e1 efs tts)) v) &&
-        efield_denote Delta efs gfs &&
+        local (tc_efield Delta efs) &&
+        efield_denote efs gfs &&
         (`(field_at sh t_root gfs v') (eval_LR e1 lr) * TT) ->
       semax Delta (|>PROPx P (LOCALx Q (SEPx R))) 
         (Sset id (nested_efield e1 efs tts))
@@ -614,6 +629,8 @@ Proof.
   + eapply derives_trans; [exact H3|].
     instantiate (1:=sh).
     instantiate (1:=e).
+    rewrite (andp_comm _ (_ * _)).
+    rewrite !andp_assoc.
     rewrite (add_andp _ _ (typeof_nested_efield _ _ _ _ _ _ _ lr H1)).
     simpl; intro rho; normalize.
     rewrite field_at_isptr.
@@ -621,13 +638,13 @@ Proof.
     normalize.
     pose proof (eval_lvalue_nested_efield Delta e t_root e1 efs gfs tts lr H1 rho).
     pose proof (tc_lvalue_nested_efield Delta e t_root e1 efs gfs tts lr H1 rho).
-    normalize in H8.
     normalize in H9.
-    rewrite (add_andp _ _ H8).
+    normalize in H10.
     rewrite (add_andp _ _ H9).
+    rewrite (add_andp _ _ H10).
     normalize.
-    rewrite H10.
-    apply andp_left2.
+    rewrite H11.
+    apply andp_left1.
     apply derives_refl.
 Qed.
 
@@ -643,7 +660,8 @@ Lemma semax_max_path_field_cast_load_37':
       PROPx P (LOCALx (tc_environ Delta :: Q) (SEPx R)) |-- 
         local (tc_LR Delta e1 lr) &&
         local (`(tc_val t (eval_cast (typeof (nested_efield e1 efs tts)) t v))) &&
-        efield_denote Delta efs gfs &&
+        local (tc_efield Delta efs) &&
+        efield_denote efs gfs &&
         (`(field_at sh t_root gfs v') (eval_LR e1 lr) * TT) ->
       semax Delta (|> PROPx P (LOCALx Q (SEPx R)))
         (Sset id (Ecast (nested_efield e1 efs tts) t))
@@ -658,6 +676,8 @@ Proof.
   + eapply derives_trans; [exact H3|].
     instantiate (1:=sh).
     instantiate (1:=e).
+    rewrite (andp_comm _ (_ * _)).
+    rewrite !andp_assoc.
     rewrite (add_andp _ _ (typeof_nested_efield _ _ _ _ _ _ _ lr H1)).
     simpl; intro rho; normalize.
     rewrite field_at_isptr.
@@ -665,13 +685,13 @@ Proof.
     normalize.
     pose proof (eval_lvalue_nested_efield Delta e t_root e1 efs gfs tts lr H1 rho).
     pose proof (tc_lvalue_nested_efield Delta e t_root e1 efs gfs tts lr H1 rho).
-    normalize in H8.
     normalize in H9.
-    rewrite (add_andp _ _ H8).
+    normalize in H10.
     rewrite (add_andp _ _ H9).
+    rewrite (add_andp _ _ H10).
     normalize.
-    rewrite H10.
-    apply andp_left2.
+    rewrite H11.
+    apply andp_left1.
     apply derives_refl.
 Qed.
 
@@ -704,8 +724,9 @@ Lemma semax_max_path_field_store_nth:
       writable_share sh ->
       PROPx P (LOCALx (tc_environ Delta :: Q) (SEPx R)) |--
         local (tc_LR Delta e1 lr) && 
-        efield_denote Delta efs gfs &&
-        local (tc_expr Delta (Ecast e2 t)) ->
+        local (tc_efield Delta efs) &&
+        efield_denote efs gfs &&
+                local (tc_expr Delta (Ecast e2 t)) ->
       semax Delta (|>PROPx P (LOCALx Q (SEPx R))) 
         (Sassign (nested_efield e1 efs tts) e2)
           (normal_ret_assert
@@ -762,12 +783,12 @@ Proof.
         pose proof (eval_lvalue_nested_efield Delta e t_root e1 efs gfs tts lr H1 rho).
         pose proof (tc_lvalue_nested_efield Delta e t_root e1 efs gfs tts lr H1 rho).
         pose proof (typeof_nested_efield _ Delta t_root _ efs _ _ lr H1 rho).
-        normalize in H13.
         normalize in H14.
-        rewrite (add_andp _ _ H13).
+        normalize in H15.
+        normalize in H16.
         rewrite (add_andp _ _ H14).
         rewrite (add_andp _ _ H15).
-        normalize.
+        rewrite (add_andp _ _ H16).
         normalize.
     } Unfocus.
     rewrite (add_andp _ _ H7).
