mc_reify/bool_funcs.v
@@ -2,6 +2,7 @@ Require Import veric.expr.
 Require Import veric.SeparationLogic.
 Require Import floyd.local2ptree.
 Require Import floyd.client_lemmas.
+Require Import floyd.loadstore_field_at.
 Require Import Coq.Bool.Bool.
 Require Import Coq.Lists.List.
 
@@ -41,6 +42,30 @@ unfold tc_temp_id, tc_temp_id_b_norho in *.
 induction (typecheck_temp_id id t Delta e); simpl in *; unfold_lift; simpl; auto; try congruence.
 rewrite andb_true_iff in *. intuition.
 rewrite orb_true_iff in *. intuition.
+Qed.
+
+Fixpoint tc_efield_b_norho Delta efs :=
+  match efs with
+  | nil => true
+  | eArraySubsc ei :: efs' =>
+      (tc_expr_b_norho Delta ei && tc_efield_b_norho Delta efs')%bool
+  | eStructField _ :: efs' => tc_efield_b_norho Delta efs'
+  | eUnionField _ :: efs' => tc_efield_b_norho Delta efs'
+  end.
+
+Lemma tc_efield_b_sound: forall efs Delta rho,
+  tc_efield_b_norho Delta efs = true -> tc_efield Delta efs rho.
+Proof.
+  intros.
+  induction efs.
+  + simpl; auto.
+  + destruct a; simpl in H |- *.
+    - apply andb_true_iff in H.
+      destruct H.
+      apply tc_expr_b_sound with (rho := rho) in H.
+      tauto.
+    - tauto.
+    - tauto.
 Qed.
 
 Definition localD (temps : PTree.t val) (locals : PTree.t (type * val)) :=
