mc_reify/set_load_store.v
@@ -1,4 +1,5 @@
-Require Import floyd.proofauto. 
+Require Import floyd.proofauto.
+Require Import JMeq.
 Require Import mc_reify.bool_funcs.
 Local Open Scope logic.
 
@@ -29,3 +30,187 @@ Proof.
   normalize.
   apply SC_remove_subst.
 Qed.
+
+Definition msubst_eval_LR T1 T2 e lr :=
+  match lr with
+  | LLLL => msubst_eval_lvalue T1 T2 e
+  | RRRR => msubst_eval_expr T1 T2 e
+  end.
+
+Fixpoint msubst_efield_denote T1 T2 (efs: list efield) : option (list gfield) :=
+  match efs with
+  | nil => Some nil
+  | eArraySubsc ei :: efs' =>
+    match typeof ei, msubst_eval_expr T1 T2 ei with
+    | Tint _ _ _, Some (Vint i) =>
+      option_map (cons (ArraySubsc (Int.unsigned i))) (msubst_efield_denote T1 T2 efs')
+    | _, _ => None
+    end
+  | eStructField i :: efs' =>
+    option_map (cons (StructField i)) (msubst_efield_denote T1 T2 efs')
+  | eUnionField i :: efs' =>
+    option_map (cons (UnionField i)) (msubst_efield_denote T1 T2 efs')
+  end.
+
+Lemma msubst_efield_denote_equiv: forall Delta P T1 T2 R efs gfs,
+  msubst_efield_denote T1 T2 efs = Some gfs ->
+  (local (tc_environ Delta)) && assertD P (localD T1 T2) R |-- efield_denote efs gfs.
+Proof.
+  intros.
+  revert gfs H; induction efs; intros.
+  + simpl in H.
+    inversion H.
+    apply prop_right.
+    auto.
+Opaque andp.
+  + destruct a;
+    simpl in H;
+    simpl efield_denote.
+Transparent andp.
+    - destruct (typeof i); try solve [inversion H].
+      destruct (msubst_eval_expr T1 T2 i) eqn:?H; [| inversion H].
+      destruct v; try solve [inversion H].
+      apply msubst_eval_expr_eq with (P := P) (Q := nil) (R := map liftx R) in H0.
+      destruct (msubst_efield_denote T1 T2 efs) eqn:?H; [| inversion H].
+      inversion H.
+      rewrite (add_andp _ _ (IHefs l eq_refl)).
+      unfold assertD, localD.
+      rewrite (add_andp _ _ H0).
+      apply andp_derives; [| auto].
+      apply andp_left2.
+      apply andp_left2.
+      rewrite Int.repr_unsigned.
+      repeat apply andp_right; auto.
+      entailer!.
+    - destruct (msubst_efield_denote T1 T2 efs) eqn:?H; [| inversion H].
+      inversion H. 
+      rewrite (add_andp _ _ (IHefs l eq_refl)).
+      apply andp_derives; [| auto].
+      entailer!.
+    - destruct (msubst_efield_denote T1 T2 efs) eqn:?H; [| inversion H].
+      inversion H. 
+      rewrite (add_andp _ _ (IHefs l eq_refl)).
+      apply andp_derives; [| auto].
+      entailer!.
+Qed.
+
+Lemma semax_PTree_load:
+  forall {Espec: OracleKind},
+    forall Delta sh e n id P T1 T2 R Rn (e1: expr)
+      (t t_root: type) (efs0 efs1: list efield) (gfs0 gfs1: list gfield) (tts0 tts1: list type)
+      (p: val) (v : val) (v' : reptype (nested_field_type2 t_root gfs0)) lr,
+      typeof_temp Delta id = Some t ->
+      is_neutral_cast (typeof (nested_efield e1 (efs1 ++ efs0) (tts1 ++ tts0))) t = true ->
+      length efs1 = length tts1 ->
+      length gfs1 = length tts1 ->
+      legal_nested_efield e t_root e1 (gfs1 ++ gfs0) (tts1 ++ tts0) lr = true ->
+      nth_error R n = Some Rn ->
+      msubst_eval_LR T1 T2 e1 lr = Some p ->
+      msubst_efield_denote T1 T2 (efs1 ++ efs0) = Some (gfs1 ++ gfs0) ->
+      (local (tc_environ Delta)) && (assertD P (localD T1 T2) (Rn :: nil)) |--
+        `(field_at sh t_root gfs0 v' p) ->
+      JMeq (proj_reptype (nested_field_type2 t_root gfs0) gfs1 v') v ->
+      (local (tc_environ Delta)) && (assertD P (localD T1 T2) R) |--
+        local (tc_LR Delta e1 lr) &&
+        local `(tc_val (typeof (nested_efield e1 (efs1 ++ efs0) (tts1 ++ tts0))) v) &&
+        local (tc_efield Delta (efs1 ++ efs0)) ->
+      (local (tc_environ Delta)) && (assertD P (localD T1 T2) R) |--
+        (!! legal_nested_field t_root (gfs1 ++ gfs0)) ->
+      semax Delta (|>assertD P (localD T1 T2) R) 
+        (Sset id (nested_efield e1 (efs1 ++ efs0) (tts1 ++ tts0)))
+          (normal_ret_assert
+            (assertD P (localD (PTree.set id v T1) T2) R)).
+Proof.
+  intros.
+  unfold assertD, localD in *.
+  rewrite insert_local in H7, H9, H10.
+  eapply semax_post'.
+  Focus 2. {
+    eapply semax_SC_field_load with (n0 := n); eauto.
+    + apply map_nth_error, H4.
+    + rewrite <- insert_local.
+      apply andp_left2.
+      destruct lr;
+      unfold eval_LR;
+      unfold msubst_eval_LR in H5.
+      - apply msubst_eval_lvalue_eq, H5.
+      - apply msubst_eval_expr_eq, H5.
+    + rewrite <- insert_local.
+      apply msubst_efield_denote_equiv, H6.
+  } Unfocus.
+  normalize.
+  apply SC_remove_subst.
+Qed.
+
+Lemma semax_PTree_cast_load:
+  forall {Espec: OracleKind},
+    forall Delta sh e n id P T1 T2 R Rn (e1: expr)
+      (t t_root: type) (efs0 efs1: list efield) (gfs0 gfs1: list gfield) (tts0 tts1: list type)
+      (p: val) (v : val) (v' : reptype (nested_field_type2 t_root gfs0)) lr,
+      typeof_temp Delta id = Some t ->
+      type_is_by_value (typeof (nested_efield e1 (efs1 ++ efs0) (tts1 ++ tts0))) ->
+      length efs1 = length tts1 ->
+      length gfs1 = length tts1 ->
+      legal_nested_efield e t_root e1 (gfs1 ++ gfs0) (tts1 ++ tts0) lr = true ->
+      nth_error R n = Some Rn ->
+      msubst_eval_LR T1 T2 e1 lr = Some p ->
+      msubst_efield_denote T1 T2 (efs1 ++ efs0) = Some (gfs1 ++ gfs0) ->
+      (local (tc_environ Delta)) && (assertD P (localD T1 T2) (Rn :: nil)) |--
+        `(field_at sh t_root gfs0 v' p) ->
+      JMeq (proj_reptype (nested_field_type2 t_root gfs0) gfs1 v') v ->
+      (local (tc_environ Delta)) && (assertD P (localD T1 T2) R) |--
+        local (tc_LR Delta e1 lr) &&
+        local (`(tc_val t (eval_cast (typeof (nested_efield e1 (efs1 ++ efs0) (tts1 ++ tts0))) t v))) &&
+        local (tc_efield Delta (efs1 ++ efs0)) ->
+      (local (tc_environ Delta)) && (assertD P (localD T1 T2) R) |--
+        (!! legal_nested_field t_root (gfs1 ++ gfs0)) ->
+      semax Delta (|>assertD P (localD T1 T2) R) 
+        (Sset id (Ecast (nested_efield e1 (efs1 ++ efs0) (tts1 ++ tts0)) t))
+          (normal_ret_assert
+            (assertD P (localD (PTree.set id (eval_cast (typeof (nested_efield e1 (efs1 ++ efs0) (tts1 ++ tts0))) t v) T1) T2) R)).
+Proof.
+  intros.
+  unfold assertD, localD in *.
+  rewrite insert_local in H7, H9, H10.
+  eapply semax_post'.
+  Focus 2. {
+    eapply semax_SC_field_cast_load with (n0 := n); eauto.
+    + apply map_nth_error, H4.
+    + rewrite <- insert_local.
+      apply andp_left2.
+      destruct lr;
+      unfold eval_LR;
+      unfold msubst_eval_LR in H5.
+      - apply msubst_eval_lvalue_eq, H5.
+      - apply msubst_eval_expr_eq, H5.
+    + rewrite <- insert_local.
+      apply msubst_efield_denote_equiv, H6.
+  } Unfocus.
+  normalize.
+  apply SC_remove_subst.
+Qed.
+
+Fixpoint tc_efield_b_norho Delta efs :=
+  match efs with
+  | nil => true
+  | eArraySubsc ei :: efs' =>
+      (tc_expr_b_norho Delta ei && tc_efield_b_norho Delta efs')%bool
+  | eStructField _ :: efs' => tc_efield_b_norho Delta efs'
+  | eUnionField _ :: efs' => tc_efield_b_norho Delta efs'
+  end.
+
+Lemma tc_efield_b_sound: forall efs Delta rho,
+  tc_efield_b_norho Delta efs = true -> tc_efield Delta efs rho.
+Proof.
+  intros.
+  induction efs.
+  + simpl; auto.
+  + destruct a; simpl in H |- *.
+    - apply andb_true_iff in H.
+      destruct H.
+      apply tc_expr_b_sound with (rho := rho) in H.
+      tauto.
+    - tauto.
+    - tauto.
+Qed.
+
